improve GEP

Phi_Semantics/PhiSem_Mem_Pointer.thy
@@ -1,5 +1,5 @@
 theory PhiSem_Mem_Pointer
-  imports PhiSem_Mem_C_Base
+  imports PhiSem_Mem_C_Base PhiSem_Agg_Void
   abbrevs "+_a" = "+\<^sub>a"
       and "|>"  = "\<^enum>"
       and "\<^enum>_a"  = "\<^enum>\<^sub>a"
@@ -26,16 +26,25 @@ subsubsection \<open>Formalization Definitions\<close>
 paragraph \<open>Base Representation for Logical and Physical Addresses\<close>
 
 declare [[typedef_overloaded]]
-datatype segidx = Null | Segment nat \<comment> \<open>nonce\<close> (layout: TY)
+datatype memblk = Null | MemBlk nat \<comment> \<open>id\<close> TY
 
-hide_const (open) layout
+setup \<open>Sign.mandatory_path "memblk"\<close>
+
+definition \<open>layout blk = (case blk of Null \<Rightarrow> void | MemBlk _ TY \<Rightarrow> TY)\<close>
+
+lemma layout[simp]:
+  \<open>memblk.layout Null = void\<close>
+  \<open>memblk.layout (MemBlk i TY) = TY\<close>
+  unfolding memblk.layout_def by simp+
+
+setup \<open>Sign.parent_path\<close>
 
 (*TODO: rename: block, offset*)
-datatype 'index memaddr = memaddr (segment: segidx) (index: 'index) (infixl "|:" 60)
+datatype 'index memaddr = memaddr (blk: memblk) (index: 'index) (infixl "|:" 60)
 declare [[typedef_overloaded = false]]
 
 declare memaddr.sel[iff]
-hide_const (open) segment index
+hide_const (open) blk index
 
 lemma split_memaddr_all: \<open>All P \<longleftrightarrow> (\<forall>blk ofs. P (memaddr blk ofs))\<close> by (metis memaddr.exhaust) 
 lemma split_memaddr_ex : \<open>Ex P  \<longleftrightarrow> (\<exists>blk ofs. P (memaddr blk ofs))\<close> by (metis memaddr.exhaust) 
@@ -48,7 +57,7 @@ proof
 next
   fix x
   assume \<open>\<And>blk ofs. PROP P (blk |: ofs)\<close>
-  note this[of \<open>memaddr.segment x\<close> \<open>memaddr.index x\<close>, simplified]
+  note this[of \<open>memaddr.blk x\<close> \<open>memaddr.index x\<close>, simplified]
   then show \<open>PROP P x\<close> .
 qed
 
@@ -78,8 +87,8 @@ type_synonym rawaddr = \<open>size_t memaddr\<close> \<comment> \<open>physical 
 
 subsubsection \<open>Algebraic Properties\<close>
 
-instantiation segidx :: zero begin
-definition [simp]: "zero_segidx = Null"
+instantiation memblk :: zero begin
+definition [simp]: "zero_memblk = Null"
 instance ..
 end
 
@@ -87,6 +96,15 @@ instantiation memaddr :: (zero) zero begin
 definition "zero_memaddr = (0 |: 0)"
 instance ..
 end
+
+lemma memaddr_blk_zero[simp]:
+  \<open>memaddr.blk 0 = Null\<close>
+  unfolding zero_memaddr_def by simp
+
+lemma memaddr_idx_zero[simp]:
+  \<open>memaddr.index 0 = 0\<close>
+  unfolding zero_memaddr_def by simp
+
 
 paragraph \<open>Freshness\<close>
 
@@ -102,22 +120,22 @@ proof
   then show False by presburger
 qed
 
-lemma segidx_infinite[simp]:
-  \<open>infinite (UNIV :: segidx set)\<close>
-  using inj_on_finite[where A = \<open>UNIV::nat set\<close> and B = \<open>(UNIV :: segidx set)\<close>
-        and f = \<open>\<lambda>n. Segment n undefined\<close>]
-  by (meson infinite_UNIV_char_0 injI segidx.inject top_greatest)
+lemma memblk_infinite[simp]:
+  \<open>infinite (UNIV :: memblk set)\<close>
+  using inj_on_finite[where A = \<open>UNIV::nat set\<close> and B = \<open>(UNIV :: memblk set)\<close>
+        and f = \<open>\<lambda>n. MemBlk n undefined\<close>]
+  by (meson infinite_UNIV_char_0 injI memblk.inject top_greatest)
 
-lemma segidx_infinite_TY:
-  \<open>infinite {a. segidx.layout a = TY}\<close>
-  using inj_on_finite[where A = \<open>UNIV::nat set\<close> and B = \<open>{a. segidx.layout a = TY}\<close>
-        and f = \<open>\<lambda>n. Segment n TY\<close>]
+lemma memblk_infinite_TY:
+  \<open>infinite {a. memblk.layout a = TY}\<close>
+  using inj_on_finite[where A = \<open>UNIV::nat set\<close> and B = \<open>{a. memblk.layout a = TY}\<close>
+        and f = \<open>\<lambda>n. MemBlk n TY\<close>]
   using inj_def by fastforce
 
 lemma Mem_freshness:
-  \<open>finite (dom f) \<Longrightarrow> \<exists>k. f k = None \<and> segidx.layout k = TY\<close>
+  \<open>finite (dom f) \<Longrightarrow> \<exists>k. f k = None \<and> memblk.layout k = TY\<close>
   unfolding dom_def
-  by (smt (verit, del_insts) Collect_mono finite_Collect_disjI finite_subset segidx_infinite_TY)
+  by (smt (verit, del_insts) Collect_mono finite_Collect_disjI finite_subset memblk_infinite_TY)
 
 
 
@@ -126,28 +144,28 @@ subsubsection \<open>Validity of Mem Block and Addresses\<close>
 abbreviation \<open>type_storable_in_mem T \<equiv> MemObj_Size T < 2^addrspace_bits\<close>
   \<comment> \<open>the size of type \<open>T\<close> is representable / less than the cap size of address space\<close>
 
-definition \<open>Valid_Segment seg = (
+definition \<open>Valid_MemBlk seg = (
     case seg of Null \<Rightarrow> True
-              | Segment _ ty \<Rightarrow> type_storable_in_mem ty
+              | MemBlk _ ty \<Rightarrow> type_storable_in_mem ty
     )\<close>
 
-lemma Valid_Segment_zero[simp]: \<open>Valid_Segment Null\<close>
-  unfolding Valid_Segment_def zero_segidx_def by simp
+lemma Valid_MemBlk_zero[simp]: \<open>Valid_MemBlk Null\<close>
+  unfolding Valid_MemBlk_def zero_memblk_def by simp
 
 abbreviation valid_rawaddr :: \<open>rawaddr \<Rightarrow> bool\<close>
-  where \<open>valid_rawaddr addr \<equiv> Valid_Segment (memaddr.segment addr)\<close>
+  where \<open>valid_rawaddr addr \<equiv> Valid_MemBlk (memaddr.blk addr)\<close>
 
 definition valid_logaddr :: "logaddr \<Rightarrow> bool"
   where "valid_logaddr addr \<longleftrightarrow>
-    Valid_Segment (memaddr.segment addr) \<and>
-    (memaddr.segment addr = Null \<longrightarrow> memaddr.index addr = []) \<and>
-    valid_index (segidx.layout (memaddr.segment addr)) (memaddr.index addr)"
+    Valid_MemBlk (memaddr.blk addr) \<and>
+    (memaddr.blk addr = Null \<longrightarrow> memaddr.index addr = []) \<and>
+    valid_index (memblk.layout (memaddr.blk addr)) (memaddr.index addr)"
 
-lemma valid_rawaddr_0[simp]: \<open>valid_rawaddr (0 |: 0)\<close>
-  by (simp add: zero_prod_def Valid_Segment_def zero_memaddr_def zero_segidx_def)
+lemma valid_rawaddr_0[simp]: \<open>valid_rawaddr 0\<close>
+  by (simp add: zero_prod_def Valid_MemBlk_def zero_memaddr_def)
 
-lemma valid_logaddr_0[simp]: \<open>valid_logaddr (0 |: [])\<close>
-  by (simp add: valid_logaddr_def zero_prod_def Valid_Segment_def zero_memaddr_def zero_segidx_def)
+lemma valid_logaddr_0[simp]: \<open>valid_logaddr 0\<close>
+  by (simp add: valid_logaddr_def zero_prod_def Valid_MemBlk_def zero_memaddr_def)
 
 
 subsubsection \<open>Basic Operations and Properties of Addresses\<close>
@@ -156,40 +174,39 @@ paragraph \<open>Size of Memory Object\<close>
 
 lemma MemObj_Size_LE_idx:
   \<open>valid_index T (base@idx) \<Longrightarrow> MemObj_Size (index_type (base@idx) T) \<le> MemObj_Size (index_type base T)\<close>
-  apply (induct base arbitrary: T idx; simp)
-  subgoal for T idx apply (induct idx arbitrary: T; simp)
-    using memobj_size_step order.trans by blast .
+  by (induct base arbitrary: T idx; simp)
 
 lemmas MemObj_Size_LE_idx_0 = MemObj_Size_LE_idx[where base = "[]", simplified]
 
 lemma index_type_type_storable_in_mem:
   \<open>type_storable_in_mem T \<Longrightarrow> valid_index T idx \<Longrightarrow> type_storable_in_mem (index_type idx T)\<close>
-  using MemObj_Size_LE_idx_0 order.strict_trans1 by blast 
+  by simp
 
 
 paragraph \<open>The type of the object that a pointer points to\<close>
 
 abbreviation logaddr_type :: \<open>logaddr \<Rightarrow> TY\<close>
-  where \<open>logaddr_type addr \<equiv> index_type (memaddr.index addr) (segidx.layout (memaddr.segment addr))\<close>
+  where \<open>logaddr_type addr \<equiv> index_type (memaddr.index addr) (memblk.layout (memaddr.blk addr))\<close>
 
 lemma logaddr_storable_in_mem:
-  \<open>valid_logaddr addr \<Longrightarrow> addr \<noteq> 0 \<Longrightarrow> type_storable_in_mem (logaddr_type addr)\<close>
-  unfolding valid_logaddr_def Valid_Segment_def zero_memaddr_def
-  apply (cases addr; simp)
-  subgoal for seg idx by (cases seg; simp add: index_type_type_storable_in_mem) .
+  \<open>valid_logaddr addr \<Longrightarrow> type_storable_in_mem (logaddr_type addr)\<close>
+  unfolding valid_logaddr_def Valid_MemBlk_def zero_memaddr_def
+  by (cases addr; simp)
+
+
 
 paragraph \<open>Relation between Logical Address and Physical Address\<close>
 
 definition logaddr_to_raw :: \<open>logaddr \<Rightarrow> rawaddr\<close>
   where \<open>logaddr_to_raw addr =
-    (case addr of seg |: idx \<Rightarrow> seg |: to_size_t (index_offset (segidx.layout seg) idx))\<close>
+    (case addr of seg |: idx \<Rightarrow> seg |: to_size_t (index_offset (memblk.layout seg) idx))\<close>
 
 lemma logaddr_to_raw_0[simp]:
   \<open>logaddr_to_raw (0 |: []) = (0 |: 0)\<close>
   unfolding logaddr_to_raw_def by simp
 
-lemma logaddr_to_raw_segment[simp]:
-  \<open>memaddr.segment (logaddr_to_raw addr) = memaddr.segment addr\<close>
+lemma logaddr_to_raw_MemBlk[simp]:
+  \<open>memaddr.blk (logaddr_to_raw addr) = memaddr.blk addr\<close>
   unfolding logaddr_to_raw_def by (cases addr) simp
 
 lemma valid_logaddr_rawaddr [simp]:
@@ -296,8 +313,9 @@ lemma logaddr_to_raw_inj:
      \<not> phantom_mem_semantic_type (logaddr_type addr1) \<Longrightarrow>
      logaddr_to_raw addr1 = logaddr_to_raw addr2 \<longrightarrow> addr1 = addr2\<close>
   unfolding logaddr_to_raw_def valid_logaddr_def
-  apply (cases addr1; cases addr2; simp)
-  by (smt (verit, ccfv_SIG) Valid_Segment_def add_leD1 index_offset_inj index_offset_upper_bound_0 len_of_addr_cap_def order_le_less_trans segidx.case_eq_if take_bit_nat_eq_self_iff word_of_nat_eq_iff)
+  by (cases addr1; cases addr2; simp; case_tac x1; case_tac x1a; simp;
+      metis Valid_MemBlk_def add_leD1 index_offset_inj index_offset_upper_bound_0 len_of_addr_cap_def memblk.simps(5) order.strict_trans1 take_bit_nat_eq_self_iff word_of_nat_eq_iff)
+  
 
 definition \<open>rawaddr_to_log T raddr = (@laddr. logaddr_to_raw laddr = raddr \<and> logaddr_type laddr = T \<and> valid_logaddr laddr)\<close>
 
@@ -324,8 +342,8 @@ notation shift_addr (infixl "||+" 60) (*depreciated!*)
 
 lemma mem_shift_shift[simp]: "a +\<^sub>a i +\<^sub>a j = a +\<^sub>a (i + j)" by (cases a) (simp add: add.assoc)
 
-lemma memaddr_segment_shift[simp]:
-  \<open>memaddr.segment (a +\<^sub>a i) = memaddr.segment a\<close>
+lemma memaddr_MemBlk_shift[simp]:
+  \<open>memaddr.blk (a +\<^sub>a i) = memaddr.blk a\<close>
   by (cases a, simp)
 
 lemma memaddr_index_shift[simp]:
@@ -368,7 +386,7 @@ TODO ...
 
 
 lemma addr_gep_memblk[iff]:
-  \<open>memaddr.segment (addr \<^enum>\<^sub>a LOGIC_IDX(i)) = memaddr.segment addr\<close>
+  \<open>memaddr.blk (addr \<^enum>\<^sub>a LOGIC_IDX(i)) = memaddr.blk addr\<close>
   unfolding addr_gep_def by (cases addr; simp)
 
 lemma addr_gep_path[iff]:
@@ -402,13 +420,13 @@ paragraph \<open>Install Memory\<close>
 
 setup \<open>Sign.mandatory_path "RES"\<close>
 
-type_synonym mem = \<open>segidx \<rightharpoonup> VAL nosep\<close>
+type_synonym mem = \<open>memblk \<rightharpoonup> VAL nosep\<close>
 
 setup \<open>Sign.parent_path\<close>
 
 resource_space aggregate_mem =
-  aggregate_mem :: \<open>{h::RES.mem. finite (dom h) \<and> (\<forall>seg \<in> dom h. h seg \<in> Some ` nosep ` Well_Type (segidx.layout seg))}\<close>
-  (aggregate_mem_resource \<open>segidx.layout\<close>)
+  aggregate_mem :: \<open>{h::RES.mem. finite (dom h) \<and> (\<forall>seg \<in> dom h. h seg \<in> Some ` nosep ` Well_Type (memblk.layout seg))}\<close>
+  (aggregate_mem_resource \<open>memblk.layout\<close>)
   by (standard; simp)
 
 
@@ -421,13 +439,13 @@ debt_axiomatization V_pointer :: \<open>rawaddr value_entry\<close>
 
 interpretation c_mem_val VAL_CONS_OF \<open>TYPE(VAL_N)\<close> \<open>TYPE(VAL)\<close> V_pointer using c_mem_val_ax .
 
-definition In_Mem :: \<open> resource \<Rightarrow> segidx \<Rightarrow> bool \<close>
+definition In_Mem :: \<open> resource \<Rightarrow> memblk \<Rightarrow> bool \<close>
   where \<open>In_Mem res seg \<equiv> seg \<in> dom (RES.aggregate_mem.get res)\<close>
 
 debt_axiomatization
     can_eqcmp_ptr[simp]: "Can_EqCompare res (V_pointer.mk rp1) (V_pointer.mk rp2)
-           \<longleftrightarrow> (memaddr.segment rp1 = memaddr.segment rp2) \<or> (rp1 = 0) \<or> (rp2 = 0) \<or>
-               (In_Mem res (memaddr.segment rp1) \<and> In_Mem res (memaddr.segment rp2))"
+           \<longleftrightarrow> (memaddr.blk rp1 = memaddr.blk rp2) \<or> (rp1 = 0) \<or> (rp2 = 0) \<or>
+               (In_Mem res (memaddr.blk rp1) \<and> In_Mem res (memaddr.blk rp2))"
 and eqcmp_ptr[simp]: "EqCompare (V_pointer.mk rp1) (V_pointer.mk rp2) \<longleftrightarrow> rp1 = rp2"
 and zero_ptr[simp]: \<open>Zero pointer = Some (V_pointer.mk 0)\<close>
 and WT_ptr[simp]: \<open>Well_Type pointer = { V_pointer.mk addr |addr. valid_rawaddr addr }\<close>
@@ -436,7 +454,7 @@ subsubsection \<open>Syntax\<close>
 
 section \<open>\<phi>-Types for Pointer\<close>
 
-subsection \<open>Raw Pointer\<close>
+subsection \<open>Physical Pointer\<close>
 
 definition RawPointer :: "(VAL, rawaddr) \<phi>"
   where "RawPointer x = ({ V_pointer.mk x } \<s>\<u>\<b>\<j> valid_rawaddr x)"
@@ -454,7 +472,7 @@ lemma RawPointer_zero[\<phi>reason 1200]:
   unfolding \<phi>Zero_def by (simp add: \<phi>expns zero_prod_def zero_memaddr_def)
 
 lemma RawPointer_eqcmp[\<phi>reason 1200]:
-  "\<phi>Equal RawPointer (\<lambda>x y. x = 0 |: 0 \<or> y = 0 |: 0 \<or> memaddr.segment x = memaddr.segment y) (=)"
+  "\<phi>Equal RawPointer (\<lambda>x y. x = 0 |: 0 \<or> y = 0 |: 0 \<or> memaddr.blk x = memaddr.blk y) (=)"
   unfolding \<phi>Equal_def by (simp add: \<phi>expns zero_memaddr_def; blast)
 
 lemma RawPointer_semty[\<phi>reason 1200]:
@@ -463,26 +481,24 @@ lemma RawPointer_semty[\<phi>reason 1200]:
   by (simp add: \<phi>expns)
 
 
-subsubsection \<open>Typed Pointer\<close>
+subsubsection \<open>Logical Pointer\<close>
 
 definition Ptr :: "TY \<Rightarrow> (VAL, logaddr) \<phi>"
   where "Ptr TY x =
-            ({ V_pointer.mk (logaddr_to_raw x) } \<s>\<u>\<b>\<j>
-                  valid_logaddr x \<and> x \<noteq> 0 \<and> logaddr_type x = TY)" (* \<and> 0 < MemObj_Size TY *)
+            ({ V_pointer.mk (logaddr_to_raw x) } \<s>\<u>\<b>\<j> valid_logaddr x \<and> logaddr_type x = TY)"
 
 lemma Ptr_expn[\<phi>expns]:
   "v \<in> (addr \<Ztypecolon> Ptr TY) \<longleftrightarrow>
-      v = V_pointer.mk (logaddr_to_raw addr) \<and> valid_logaddr addr
-    \<and> addr \<noteq> 0 \<and> logaddr_type addr = TY" (* \<and> 0 < MemObj_Size TY *)
+      v = V_pointer.mk (logaddr_to_raw addr) \<and> valid_logaddr addr \<and> logaddr_type addr = TY"
   unfolding \<phi>Type_def by (simp add: Ptr_def Subjection_expn)
 
 lemma Ptr_inhabited[elim!, \<phi>inhabitance_rule]:
   "Inhabited (addr \<Ztypecolon> Ptr TY) \<Longrightarrow>
-      (valid_logaddr addr \<and> addr \<noteq> 0 \<and> logaddr_type addr = TY \<Longrightarrow> C) \<Longrightarrow> C"
+      (valid_logaddr addr \<and> logaddr_type addr = TY \<Longrightarrow> C) \<Longrightarrow> C"
   unfolding Inhabited_def by (simp add: \<phi>expns)
 
 lemma Ptr_eqcmp[\<phi>reason 1000]:
-    "\<phi>Equal (Ptr TY) (\<lambda>x y. memaddr.segment x = memaddr.segment y \<and> \<not> phantom_mem_semantic_type TY) (=)"
+    "\<phi>Equal (Ptr TY) (\<lambda>x y. memaddr.blk x = memaddr.blk y \<and> \<not> phantom_mem_semantic_type TY) (=)"
   unfolding \<phi>Equal_def
   by (simp add: \<phi>expns) (metis logaddr_to_raw_inj)
 
@@ -505,10 +521,30 @@ proc op_get_element_pointer_symbol:
   semantic_return \<open>
      V_pointer.mk (logaddr_to_raw (rawaddr_to_log TY (V_pointer.dest (\<phi>arg.dest \<a>\<r>\<g>1)) \<^enum>\<^sub>a LOGIC_SYMBOL(symbol)))
          \<in> (addr \<^enum>\<^sub>a LOGIC_SYMBOL(symbol) \<Ztypecolon> Ptr TY')\<close>
-      certified by ((insert useful, simp add: \<phi>expns, cases \<open>phantom_mem_semantic_type (logaddr_type addr)\<close>;
-                     simp add: logaddr_to_raw_phantom_mem_type),
-                   smt (verit, del_insts) logaddr_to_raw_phantom_mem_type logaddr_to_raw_segment rawaddr_to_log_def someI_ex,
+     certified by ((insert useful, simp add: \<phi>expns,
+                   cases \<open>phantom_mem_semantic_type (logaddr_type addr)\<close>;
+                   cases \<open>addr = 0\<close>;
+                   simp add: logaddr_to_raw_phantom_mem_type),
+                   (insert valid_idx_step_void, force)[1],
+                   smt (verit, del_insts) logaddr_to_raw_phantom_mem_type logaddr_to_raw_MemBlk rawaddr_to_log_def someI_ex,
+                   (insert valid_idx_step_void, force)[1],
                    fastforce)
+\<medium_right_bracket> .
+
+proc op_get_element_pointer_const_numidx:
+  requires \<open>Is_Literal i\<close>
+       and \<open>\<c>\<o>\<n>\<d>\<i>\<t>\<i>\<o>\<n>[eval_aggregate_path] valid_idx_step TY AG_IDX(#i)\<close>
+       and \<open> \<s>\<i>\<m>\<p>\<l>\<i>\<f>\<y>[eval_aggregate_path] TY' : idx_step_type AG_IDX(#i) TY\<close>
+  input  \<open>addr \<Ztypecolon> \<v>\<a>\<l> Ptr TY\<close>
+  output \<open>addr \<^enum>\<^sub>a #i \<Ztypecolon> \<v>\<a>\<l> Ptr TY'\<close>
+\<medium_left_bracket>
+  $addr semantic_local_value pointer
+  semantic_return \<open>
+     V_pointer.mk (logaddr_to_raw (rawaddr_to_log TY (V_pointer.dest (\<phi>arg.dest \<a>\<r>\<g>1)) \<^enum>\<^sub>a LOGIC_IDX(AgIdx_N i)))
+         \<in> (addr \<^enum>\<^sub>a LOGIC_IDX(AgIdx_N i) \<Ztypecolon> Ptr TY')\<close>
+    certified by ((insert useful, simp add: \<phi>expns; cases \<open>addr = 0\<close>; simp),
+                  (insert valid_idx_step_void, force)[1],
+                  smt logaddr_to_raw_phantom_mem_type rawaddr_to_log rawaddr_to_log_def someI_ex)
 \<medium_right_bracket> .
 
 
