Phi_Semantics/PhiSem_Agg_Void.thy
@@ -1,0 +1,9 @@
+theory PhiSem_Agg_Void
+  imports PhiSem_Aggregate_Base PhiSem_Void
+begin
+
+debt_axiomatization
+    valid_idx_step_void[eval_aggregate_path] : \<open>valid_idx_step void i \<longleftrightarrow> False\<close>
+
+
+end
